Add particular pattern for "always" and add proofs for "Revolving door"

examples/RevolvingDoor/Requirements.thy
@@ -1,5 +1,5 @@
 theory Requirements
-  imports "../Derived_Patterns"  RevolvingDoor
+  imports "../Derived_Patterns"  CommonExtraInv
 begin
 
 (*
@@ -21,8 +21,18 @@ definition R1 where "R1 s \<equiv> toEnvP s \<and>
 always2_part (\<lambda> s1. getVarBool s1 rotation' = False) (\<lambda> s2. getVarBool s2 user' \<and> \<not> getVarBool s2 pressure')
 (\<lambda> s2. getVarBool s2 rotation' = True) s"
 
+definition Einv1 where "Einv1 s \<equiv> commonExtraInv s \<and> 
+always2_inv_part (\<lambda> s. getPstate s Controller' = Controller'rotating')
+ (\<lambda> s1. getVarBool s1 rotation' = False) (\<lambda> s2. getVarBool s2 user' \<and> \<not> getVarBool s2 pressure')
+(\<lambda> s2. getVarBool s2 rotation' = True) s"
+
 definition R2 where "R2 s \<equiv> toEnvP s \<and> 
 always2_part (\<lambda> s1. getVarBool s1 rotation' = True) (\<lambda> s2. getVarBool s2 user' \<and> \<not> getVarBool s2 pressure')
+(\<lambda> s2. getVarBool s2 rotation' = True) s"
+
+definition Einv2 where "Einv2 s \<equiv> commonExtraInv s \<and> 
+always2_inv_part (\<lambda> s. getPstate s Controller' \<noteq> Controller'rotating')
+ (\<lambda> s1. getVarBool s1 rotation' = True) (\<lambda> s2. getVarBool s2 user' \<and> \<not> getVarBool s2 pressure')
 (\<lambda> s2. getVarBool s2 rotation' = True) s"
 
 definition R3 where "R3 s \<equiv> toEnvP s \<and>
@@ -30,20 +40,39 @@ P1_2_part DELAY'TIMEOUT (\<lambda> s1. getVarBool s1 rotation' = True) (\<lambda
 (\<lambda> s3. getVarBool s3 rotation' = True \<and> getVarBool s3 user' = False) 
 (\<lambda> s3. getVarBool s3 rotation' = False \<or> getVarBool s3 user' = True) s"
 
+definition Einv3 where "Einv3 s \<equiv> commonExtraInv s \<and>
+P1_2_inv_part DELAY'TIMEOUT (\<lambda> s. getPstate s Controller' \<noteq> Controller'rotating')
+(\<lambda> s. if getPstate s Controller' = Controller'rotating' then ltime s Controller' else 0)
+ (\<lambda> s1. getVarBool s1 rotation' = True) (\<lambda> s2. getVarBool s2 user' = False)
+(\<lambda> s3. getVarBool s3 rotation' = True \<and> getVarBool s3 user' = False) 
+(\<lambda> s3. getVarBool s3 rotation' = False \<or> getVarBool s3 user' = True) s"
+
 definition R4 where "R4 s \<equiv> toEnvP s \<and> 
 P2_2_part SUSPENSION_TIME'TIMEOUT (\<lambda> s1. getVarBool s1 rotation' = True) (\<lambda> s2. getVarBool s2 pressure' = True)
 (\<lambda> s3. getVarBool s3 brake' = True) s"
 
-definition R5 where "R5 s \<equiv> toEnvP s \<and> (\<forall> s1 s2. substate s1 s2 \<and> substate s2 s \<and>
-toEnvP s1 \<and> toEnvP s2 \<and> toEnvNum s1 s2 = 1 \<and> toEnvNum s2 s \<ge> SUSPENSION_TIME'TIMEOUT \<and>
-getVarBool s1 brake \<and> \<not> getVarBool s2 pressure \<longrightarrow>
-(\<exists> s4. toEnvP s4 \<and> substate s2 s4 \<and> substate s4 s \<and> toEnvNum s2 s4 \<le> SUSPENSION_TIME'TIMEOUT \<and>
-(getVarBool s4 rotation = True \<or> getVarBool s4 pressure) \<and>
-(\<forall> s3. toEnvP s3 \<and> substate s2 s3 \<and> substate s3 s4 \<and> s3 \<noteq> s4 \<longrightarrow> getVarBool s3 rotation = False \<and> \<not> getVarBool s3 pressure)))"
+definition Einv4 where "Einv4 s \<equiv> commonExtraInv s \<and> 
+P2_2_inv_part SUSPENSION_TIME'TIMEOUT (\<lambda> s. getPstate s Controller' \<noteq> Controller'rotating')
+(\<lambda> s. if getPstate s Controller' = Controller'suspended' then ltime s Controller' - 1 else SUSPENSION_TIME'TIMEOUT -1)
+ (\<lambda> s1. getVarBool s1 rotation' = True) (\<lambda> s2. getVarBool s2 pressure' = True)
+(\<lambda> s3. getVarBool s3 brake' = True) s"
 
-definition R6 where "R6 s \<equiv> toEnvP s \<and> (\<forall> s1. substate s1 s \<and> toEnvP s1 \<and> getVarBool s1 brake \<longrightarrow>
- getVarBool s1 rotation = False)"
+definition R5 where "R5 s \<equiv> toEnvP s \<and>
+P1_2_part SUSPENSION_TIME'TIMEOUT (\<lambda> s1. getVarBool s1 brake' = True) (\<lambda> s2. getVarBool s2 pressure' = False)
+(\<lambda> s3. getVarBool s3 rotation' = False \<and> getVarBool s3 pressure' = False)
+ (\<lambda> s4. getVarBool s4 rotation' = True \<or> getVarBool s4 pressure' = True) s"
 
-definition env where "env s \<equiv> True"
+definition Einv5 where "Einv5 s \<equiv> commonExtraInv s \<and>
+P1_2_inv_part SUSPENSION_TIME'TIMEOUT (\<lambda> s. getPstate s Controller' \<noteq> Controller'suspended')
+(\<lambda> s. if getPstate s Controller' = Controller'suspended' then ltime s Controller' else 0)
+ (\<lambda> s1. getVarBool s1 brake' = True) (\<lambda> s2. getVarBool s2 pressure' = False)
+(\<lambda> s3. getVarBool s3 rotation' = False \<and> getVarBool s3 pressure' = False)
+ (\<lambda> s4. getVarBool s4 rotation' = True \<or> getVarBool s4 pressure' = True) s"
+
+definition R6 where "R6 s \<equiv> toEnvP s \<and>
+always_part (\<lambda> s1. getVarBool s1 rotation' = False \<or> getVarBool s1 brake' = False) s"
+
+definition Einv6 where "Einv6 s \<equiv> commonExtraInv s \<and>
+always_inv_part (\<lambda> s1. getVarBool s1 rotation' = False \<or> getVarBool s1 brake' = False) s"
 
 end
