examples/RevolvingDoor/CommonExtraInv_Proofs.thy
@@ -1,0 +1,67 @@
+theory CommonExtraInv_Proofs imports CommonExtraInv
+ begin
+theorem cei1: "VC1 commonExtraInv s0"
+unfolding VC1_def commonExtraInv_def
+by auto
+
+theorem cei2: "VC2 commonExtraInv env s0  user'value pressure'value"
+unfolding VC2_def commonExtraInv_def
+by force
+
+theorem cei3: "VC3 commonExtraInv env s0  user'value pressure'value"
+unfolding VC3_def commonExtraInv_def
+by force
+
+theorem cei4: "VC4 commonExtraInv env s0  user'value pressure'value"
+unfolding VC4_def commonExtraInv_def
+by force
+
+theorem cei5: "VC5 commonExtraInv env s0  user'value pressure'value"
+unfolding VC5_def commonExtraInv_def
+by force
+
+theorem cei6: "VC6 commonExtraInv env s0  user'value pressure'value"
+unfolding VC6_def commonExtraInv_def
+by force
+
+theorem cei7: "VC7 commonExtraInv env s0  user'value pressure'value"
+unfolding VC7_def commonExtraInv_def
+by force
+
+theorem cei8: "VC8 commonExtraInv env s0  user'value pressure'value"
+unfolding VC8_def commonExtraInv_def
+by force
+
+theorem cei9: "VC9 commonExtraInv env s0  user'value pressure'value"
+unfolding VC9_def commonExtraInv_def
+by force
+
+theorem cei10: "VC10 commonExtraInv env s0  user'value pressure'value"
+unfolding VC10_def commonExtraInv_def
+by force
+
+theorem cei11: "VC11 commonExtraInv env s0  user'value pressure'value"
+unfolding VC11_def commonExtraInv_def
+by force
+
+theorem cei12: "VC12 commonExtraInv env s0  user'value pressure'value"
+unfolding VC12_def commonExtraInv_def
+by force
+
+theorem cei13: "VC13 commonExtraInv env s0  user'value pressure'value"
+unfolding VC13_def commonExtraInv_def
+by force
+
+theorem cei14: "VC14 commonExtraInv env s0  user'value pressure'value"
+unfolding VC14_def commonExtraInv_def
+by force
+
+theorem cei15: "VC15 commonExtraInv env s0  user'value pressure'value"
+unfolding VC15_def commonExtraInv_def
+by force
+
+theorem cei16: "VC16 commonExtraInv env s0  user'value pressure'value"
+unfolding VC16_def commonExtraInv_def
+by force
+
+end
