examples/RevolvingDoor/Einv4_Proofs.thy
@@ -1,0 +1,172 @@
+theory Einv4_Proofs imports Requirements CommonExtraInv_Proofs
+ begin
+theorem extra1: "VC1 Einv4 s0"
+unfolding VC1_def Einv4_def P2_2_inv_part_used_patterns commonExtraInv_def
+by auto
+
+theorem extra2: "VC2 Einv4 env s0  user'value pressure'value"
+unfolding VC2_def Einv4_def
+ apply(rule impI)
+  apply(rule conjI)
+    using cei2 apply((auto simp add: VC2_def)[1];fastforce)
+  apply(unfold commonExtraInv_def)
+  apply(erule conjE)+
+  apply(erule P2_2_inv_saving)
+   apply(auto split: if_splits)
+  done
+
+theorem extra3: "VC3 Einv4 env s0  user'value pressure'value"
+unfolding VC3_def Einv4_def
+ apply(rule impI)
+  apply(rule conjI)
+    using cei3 apply((auto simp add: VC3_def)[1];fastforce)
+  apply(unfold commonExtraInv_def)
+  apply(erule conjE)+
+  apply(erule P2_2_inv_saving)
+   apply(auto split: if_splits)
+  done
+
+theorem extra4: "VC4 Einv4 env s0  user'value pressure'value"
+unfolding VC4_def Einv4_def
+ apply(rule impI)
+  apply(rule conjI)
+    using cei4 apply((auto simp add: VC4_def)[1];fastforce)
+  apply(unfold commonExtraInv_def)
+  apply(erule conjE)+
+  apply(erule P2_2_inv_saving)
+   apply(auto split: if_splits)
+  done
+
+theorem extra5: "VC5 Einv4 env s0  user'value pressure'value"
+unfolding VC5_def Einv4_def
+ apply(rule impI)
+  apply(rule conjI)
+    using cei5 apply((auto simp add: VC5_def)[1];fastforce)
+  apply(unfold commonExtraInv_def)
+  apply(erule conjE)+
+  apply(erule P2_2_inv_saving)
+   apply(auto split: if_splits)
+  done
+
+theorem extra6: "VC6 Einv4 env s0  user'value pressure'value"
+unfolding VC6_def Einv4_def
+ apply(rule impI)
+  apply(rule conjI)
+    using cei6 apply((auto simp add: VC6_def)[1];fastforce)
+  apply(unfold commonExtraInv_def)
+  apply(erule conjE)+
+  apply(erule P2_2_inv_saving)
+   apply(auto split: if_splits)
+  done
+
+theorem extra7: "VC7 Einv4 env s0  user'value pressure'value"
+unfolding VC7_def Einv4_def
+ apply(rule impI)
+  apply(rule conjI)
+    using cei7 apply((auto simp add: VC7_def)[1];fastforce)
+  apply(unfold commonExtraInv_def)
+  apply(erule conjE)+
+  apply(erule P2_2_inv_saving)
+   apply(auto split: if_splits)
+  done
+
+theorem extra8: "VC8 Einv4 env s0  user'value pressure'value"
+unfolding VC8_def Einv4_def
+ apply(rule impI)
+  apply(rule conjI)
+    using cei8 apply((auto simp add: VC8_def)[1];fastforce)
+  apply(unfold commonExtraInv_def)
+  apply(erule conjE)+
+  apply(erule P2_2_inv_saving)
+   apply(auto split: if_splits)
+  done
+
+theorem extra9: "VC9 Einv4 env s0  user'value pressure'value"
+unfolding VC9_def Einv4_def
+ apply(rule impI)
+  apply(rule conjI)
+    using cei9 apply((auto simp add: VC9_def)[1];fastforce)
+  apply(unfold commonExtraInv_def)
+  apply(erule conjE)+
+  apply(erule P2_2_inv_saving)
+   apply(auto split: if_splits)
+  done
+
+theorem extra10: "VC10 Einv4 env s0  user'value pressure'value"
+unfolding VC10_def Einv4_def
+ apply(rule impI)
+  apply(rule conjI)
+    using cei10 apply((auto simp add: VC10_def)[1];fastforce)
+  apply(unfold commonExtraInv_def)
+  apply(erule conjE)+
+  apply(erule P2_2_inv_saving)
+   apply(auto split: if_splits)
+  done
+
+theorem extra11: "VC11 Einv4 env s0  user'value pressure'value"
+unfolding VC11_def Einv4_def
+ apply(rule impI)
+  apply(rule conjI)
+    using cei11 apply((auto simp add: VC11_def)[1];fastforce)
+  apply(unfold commonExtraInv_def)
+  apply(erule conjE)+
+  apply(erule P2_2_inv_saving)
+   apply(auto split: if_splits)
+  done
+
+theorem extra12: "VC12 Einv4 env s0  user'value pressure'value"
+unfolding VC12_def Einv4_def
+ apply(rule impI)
+  apply(rule conjI)
+    using cei12 apply((auto simp add: VC12_def)[1];fastforce)
+  apply(unfold commonExtraInv_def)
+  apply(erule conjE)+
+  apply(erule P2_2_inv_saving)
+   apply(auto split: if_splits)
+  done
+
+theorem extra13: "VC13 Einv4 env s0  user'value pressure'value"
+unfolding VC13_def Einv4_def
+ apply(rule impI)
+  apply(rule conjI)
+    using cei13 apply((auto simp add: VC13_def)[1];fastforce)
+  apply(unfold commonExtraInv_def)
+  apply(erule conjE)+
+  apply(erule P2_2_inv_saving)
+   apply(auto split: if_splits)
+  done
+
+theorem extra14: "VC14 Einv4 env s0  user'value pressure'value"
+unfolding VC14_def Einv4_def
+ apply(rule impI)
+  apply(rule conjI)
+    using cei14 apply((auto simp add: VC14_def)[1];fastforce)
+  apply(unfold commonExtraInv_def)
+  apply(erule conjE)+
+  apply(erule P2_2_inv_saving)
+   apply(auto split: if_splits)
+  done
+
+theorem extra15: "VC15 Einv4 env s0  user'value pressure'value"
+unfolding VC15_def Einv4_def
+ apply(rule impI)
+  apply(rule conjI)
+    using cei15 apply((auto simp add: VC15_def)[1];fastforce)
+  apply(unfold commonExtraInv_def)
+  apply(erule conjE)+
+  apply(erule P2_2_inv_saving)
+   apply(auto split: if_splits)
+  done
+
+theorem extra16: "VC16 Einv4 env s0  user'value pressure'value"
+unfolding VC16_def Einv4_def
+ apply(rule impI)
+  apply(rule conjI)
+    using cei16 apply((auto simp add: VC16_def)[1];fastforce)
+  apply(unfold commonExtraInv_def)
+  apply(erule conjE)+
+  apply(erule P2_2_inv_saving)
+   apply(auto split: if_splits)
+  done
+
+end
